src/SlabsCommon.fst
@@ -256,79 +256,78 @@ let p_guard_pack (#opened:_)
 
 inline_for_extraction noextract
 let slab_array
-  (slab_region: array U8.t{A.length slab_region = U32.v metadata_max * U32.v page_size})
-  (md_count: U32.t{U32.v md_count < U32.v metadata_max})
+  (slab_region: array U8.t{A.length slab_region = US.v metadata_max * U32.v page_size})
+  (md_count: US.t{US.v md_count < US.v metadata_max})
   : Pure (array U8.t)
   (requires
-    A.length slab_region = U32.v metadata_max * U32.v page_size /\
-    U32.v md_count < U32.v metadata_max)
+    A.length slab_region = US.v metadata_max * U32.v page_size /\
+    US.v md_count < US.v metadata_max)
   (ensures fun r ->
     A.length r = U32.v page_size /\
     same_base_array r slab_region /\
-    A.offset (A.ptr_of r) == A.offset (A.ptr_of slab_region) + U32.v md_count * U32.v page_size
+    A.offset (A.ptr_of r) == A.offset (A.ptr_of slab_region) + US.v md_count * U32.v page_size
   )
   =
   let ptr = A.ptr_of slab_region in
-  let shift = U32.mul md_count page_size in
-  let shift_size_t = u32_to_sz shift in
+  let page_size_t = u32_to_sz page_size in
+  let shift_size_t = US.mul md_count page_size_t in
   let ptr_shifted = A.ptr_shift ptr shift_size_t in
   (|ptr_shifted, G.hide (U32.v page_size)|)
 
 let pack_slab_array (#opened:_)
-  (slab_region: array U8.t{A.length slab_region = U32.v metadata_max * U32.v page_size})
-  (md_count: U32.t{U32.v md_count < U32.v metadata_max})
+  (slab_region: array U8.t{A.length slab_region = US.v metadata_max * U32.v page_size})
+  (md_count: US.t{US.v md_count < US.v metadata_max})
   : SteelGhost unit opened
-    (A.varray (A.split_l (A.split_r slab_region (u32_to_sz (U32.mul md_count page_size))) (u32_to_sz page_size)))
+    (A.varray (A.split_l (A.split_r slab_region (US.mul md_count (u32_to_sz page_size))) (u32_to_sz page_size)))
     (fun _ -> A.varray (slab_array slab_region md_count))
     (requires fun _ -> True)
     (ensures fun h0 _ h1 ->
-      A.asel (A.split_l (A.split_r slab_region (u32_to_sz (U32.mul md_count page_size))) (u32_to_sz page_size)) h0 ==
+      A.asel (A.split_l (A.split_r slab_region (US.mul md_count (u32_to_sz page_size))) (u32_to_sz page_size)) h0 ==
       A.asel (slab_array slab_region md_count) h1)
   = change_equal_slprop
-    (A.varray (A.split_l (A.split_r slab_region (u32_to_sz (U32.mul md_count page_size))) (u32_to_sz page_size)))
+    (A.varray (A.split_l (A.split_r slab_region (US.mul md_count (u32_to_sz page_size))) (u32_to_sz page_size)))
     (A.varray (slab_array slab_region md_count))
 
 inline_for_extraction noextract
 let md_bm_array
-  (md_bm_region: array U64.t{A.length md_bm_region = U32.v metadata_max * 4})
-  (md_count: U32.t{U32.v md_count < U32.v metadata_max})
+  (md_bm_region: array U64.t{A.length md_bm_region = US.v metadata_max * 4})
+  (md_count: US.t{US.v md_count < US.v metadata_max})
   : Pure (array U64.t)
   (requires
-    A.length md_bm_region = U32.v metadata_max * 4 /\
-    U32.v md_count < U32.v metadata_max)
+    A.length md_bm_region = US.v metadata_max * 4 /\
+    US.v md_count < US.v metadata_max)
   (ensures fun r ->
     A.length r = 4 /\
     same_base_array r md_bm_region
   )
   =
   let ptr = A.ptr_of md_bm_region in
-  let shift = U32.mul md_count 4ul in
-  let shift_size_t = u32_to_sz shift in
+  let shift_size_t = US.mul md_count 4sz in
   let ptr_shifted = A.ptr_shift ptr shift_size_t in
   (|ptr_shifted, G.hide 4|)
 
 let pack_md_bm_array (#opened:_)
-  (md_bm_region: array U64.t{A.length md_bm_region = U32.v metadata_max * 4})
-  (md_count: U32.t{U32.v md_count < U32.v metadata_max})
+  (md_bm_region: array U64.t{A.length md_bm_region = US.v metadata_max * 4})
+  (md_count: US.t{US.v md_count < US.v metadata_max})
   : SteelGhost unit opened
-    (A.varray (A.split_l (A.split_r md_bm_region (u32_to_sz (U32.mul md_count 4ul))) (u32_to_sz 4ul)))
+    (A.varray (A.split_l (A.split_r md_bm_region (US.mul md_count 4sz)) 4sz))
     (fun _ -> A.varray (md_bm_array md_bm_region md_count))
     (requires fun _ -> True)
     (ensures fun h0 _ h1 ->
-      A.asel (A.split_l (A.split_r md_bm_region (u32_to_sz (U32.mul md_count 4ul))) (u32_to_sz 4ul)) h0 ==
+      A.asel (A.split_l (A.split_r md_bm_region (US.mul md_count 4sz)) 4sz) h0 ==
       A.asel (md_bm_array md_bm_region md_count) h1)
   = change_equal_slprop
-    (A.varray (A.split_l (A.split_r md_bm_region (u32_to_sz (U32.mul md_count 4ul))) (u32_to_sz 4ul)))
+    (A.varray (A.split_l (A.split_r md_bm_region (US.mul md_count 4sz)) 4sz))
     (A.varray (md_bm_array md_bm_region md_count))
 
 inline_for_extraction noextract
 let md_array
-  (md_region: array AL.cell{A.length md_region = U32.v metadata_max})
-  (md_count: U32.t{U32.v md_count < U32.v metadata_max})
+  (md_region: array AL.cell{A.length md_region = US.v metadata_max})
+  (md_count: US.t{US.v md_count < US.v metadata_max})
   : Pure (array AL.cell)
   (requires
-    A.length md_region = U32.v metadata_max /\
-    U32.v md_count < U32.v metadata_max)
+    A.length md_region = US.v metadata_max /\
+    US.v md_count < US.v metadata_max)
   (ensures fun r ->
     A.length r = 1 /\
     same_base_array r md_region /\
@@ -336,37 +335,36 @@ let md_array
   )
   =
   let ptr = A.ptr_of md_region in
-  let shift_size_t = u32_to_sz md_count in
-  let ptr_shifted = A.ptr_shift ptr shift_size_t in
+  let ptr_shifted = A.ptr_shift ptr md_count in
   (|ptr_shifted, G.hide 1|)
 
 let pack_md_array (#opened:_)
-  (md_region: array AL.cell{A.length md_region = U32.v metadata_max})
-  (md_count: U32.t{U32.v md_count < U32.v metadata_max})
+  (md_region: array AL.cell{A.length md_region = US.v metadata_max})
+  (md_count: US.t{US.v md_count < US.v metadata_max})
   : SteelGhost unit opened
-    (A.varray (A.split_l (A.split_r md_region (u32_to_sz md_count)) (u32_to_sz 1ul)))
+    (A.varray (A.split_l (A.split_r md_region md_count) 1sz))
     (fun _ -> A.varray (md_array md_region md_count))
     (requires fun _ -> True)
     (ensures fun h0 _ h1 ->
-      A.asel (A.split_l (A.split_r md_region (u32_to_sz md_count)) (u32_to_sz 1ul)) h0 ==
+      A.asel (A.split_l (A.split_r md_region md_count) 1sz) h0 ==
       A.asel (md_array md_region md_count) h1)
   = change_equal_slprop
-      (A.varray (A.split_l (A.split_r md_region (u32_to_sz md_count)) (u32_to_sz 1ul)))
+      (A.varray (A.split_l (A.split_r md_region md_count) 1sz))
       (A.varray (md_array md_region md_count))
 
 let unpack_md_array (#opened:_)
-  (md_region: array AL.cell{A.length md_region = U32.v metadata_max})
-  (md_count: U32.t{U32.v md_count < U32.v metadata_max})
+  (md_region: array AL.cell{A.length md_region = US.v metadata_max})
+  (md_count: US.t{US.v md_count < US.v metadata_max})
   : SteelGhost unit opened
     (A.varray (md_array md_region md_count))
-    (fun _ -> A.varray (A.split_l (A.split_r md_region (u32_to_sz md_count)) 1sz))
+    (fun _ -> A.varray (A.split_l (A.split_r md_region md_count) 1sz))
     (requires fun _ -> True)
     (ensures fun h0 _ h1 ->
-      A.asel (A.split_l (A.split_r md_region (u32_to_sz md_count)) 1sz) h1 ==
+      A.asel (A.split_l (A.split_r md_region md_count) 1sz) h1 ==
       A.asel (md_array md_region md_count) h0)
   = change_equal_slprop
       (A.varray (md_array md_region md_count))
-      (A.varray (A.split_l (A.split_r md_region (u32_to_sz md_count)) 1sz))
+      (A.varray (A.split_l (A.split_r md_region md_count) 1sz))
 
 let t (size_class: sc) : Type0 =
   dtuple2
@@ -376,11 +374,11 @@ let t (size_class: sc) : Type0 =
 
 let f_lemma
   (size_class: sc)
-  (slab_region: array U8.t{A.length slab_region = U32.v metadata_max * U32.v page_size})
-  (md_bm_region: array U64.t{A.length md_bm_region = U32.v metadata_max * 4})
-  (md_count_v: U32.t{U32.v md_count_v <= U32.v metadata_max})
-  (md_region_lv: Seq.lseq AL.status (U32.v md_count_v))
-  (i: U32.t{U32.v i < U32.v md_count_v})
+  (slab_region: array U8.t{A.length slab_region = US.v metadata_max * U32.v page_size})
+  (md_bm_region: array U64.t{A.length md_bm_region = US.v metadata_max * 4})
+  (md_count_v: US.t{US.v md_count_v <= US.v metadata_max})
+  (md_region_lv: Seq.lseq AL.status (US.v md_count_v))
+  (i: US.t{US.v i < US.v md_count_v})
   : Lemma
   (t_of (f size_class slab_region md_bm_region md_count_v md_region_lv i)
   == t size_class)
@@ -392,13 +390,13 @@ let f_lemma
 let pack_3
   (#opened:_)
   (size_class: sc)
-  (slab_region: array U8.t{A.length slab_region = U32.v metadata_max * U32.v page_size})
-  (md_bm_region: array U64.t{A.length md_bm_region = U32.v metadata_max * 4})
-  (md_region: array AL.cell{A.length md_region = U32.v metadata_max})
-  (md_count: ref U32.t)
+  (slab_region: array U8.t{A.length slab_region = US.v metadata_max * U32.v page_size})
+  (md_bm_region: array U64.t{A.length md_bm_region = US.v metadata_max * 4})
+  (md_region: array AL.cell{A.length md_region = US.v metadata_max})
+  (md_count: ref US.t)
   (r1 r2 r3 r4: ref US.t)
-  (md_count_v: U32.t{U32.v md_count_v <= U32.v metadata_max})
-  (md_region_lv: G.erased (Seq.lseq AL.status (U32.v md_count_v)))
+  (md_count_v: US.t{US.v md_count_v <= US.v metadata_max})
+  (md_region_lv: G.erased (Seq.lseq AL.status (US.v md_count_v)))
   (idx1 idx2 idx3 idx4: US.t)
   : SteelGhost unit opened
   (
@@ -408,14 +406,14 @@ let pack_3
     vptr r3 `star`
     vptr r4 `star`
     (AL.varraylist pred1 pred2 pred3 pred4
-      (A.split_l md_region (u32_to_sz md_count_v))
+      (A.split_l md_region md_count_v)
       (US.v idx1) (US.v idx2) (US.v idx3) (US.v idx4)) `star`
     starseq
-      #(pos:U32.t{U32.v pos < U32.v md_count_v})
+      #(pos:US.t{US.v pos < US.v md_count_v})
       #(t size_class)
       (f size_class slab_region md_bm_region md_count_v (G.reveal md_region_lv))
       (f_lemma size_class slab_region md_bm_region md_count_v (G.reveal md_region_lv))
-      (SeqUtils.init_u32_refined (U32.v md_count_v))
+      (SeqUtils.init_us_refined (US.v md_count_v))
   )
   (fun _ ->
     vrefinedep
@@ -425,9 +423,9 @@ let pack_3
   )
   (requires fun h0 ->
     let gs0 = AL.v_arraylist pred1 pred2 pred3 pred4
-      (A.split_l md_region (u32_to_sz md_count_v))
+      (A.split_l md_region md_count_v)
       (US.v idx1) (US.v idx2) (US.v idx3) (US.v idx4) h0 in
-    U32.v md_count_v <> AL.null /\
+    US.v md_count_v <> AL.null /\
     sel md_count h0 == md_count_v /\
     sel r1 h0 == idx1 /\
     sel r2 h0 == idx2 /\
@@ -447,21 +445,24 @@ let pack_3
   =
   intro_vrefine
     (ind_varraylist_aux2 pred1 pred2 pred3 pred4
-      (A.split_l md_region (u32_to_sz md_count_v)) (((idx1, idx2), idx3), idx4))
+      (A.split_l md_region md_count_v) (((idx1, idx2), idx3), idx4))
     (ind_varraylist_aux_refinement pred1 pred2 pred3 pred4
-      (A.split_l md_region (u32_to_sz md_count_v)) (((idx1, idx2), idx3), idx4));
+      (A.split_l md_region md_count_v) (((idx1, idx2), idx3), idx4));
   intro_vdep
     (vptr r1 `star` vptr r2 `star` vptr r3 `star` vptr r4)
-    (ind_varraylist_aux pred1 pred2 pred3 pred4 (A.split_l md_region (u32_to_sz md_count_v)) (((idx1, idx2), idx3), idx4))
-    (ind_varraylist_aux pred1 pred2 pred3 pred4 (A.split_l md_region (u32_to_sz md_count_v)));
+    (ind_varraylist_aux pred1 pred2 pred3 pred4
+      (A.split_l md_region md_count_v)
+      (((idx1, idx2), idx3), idx4))
+    (ind_varraylist_aux pred1 pred2 pred3 pred4
+      (A.split_l md_region md_count_v));
 
   change_equal_slprop
     (starseq
-      #(pos:U32.t{U32.v pos < U32.v md_count_v})
+      #(pos:US.t{US.v pos < US.v md_count_v})
       #(t size_class)
       (f size_class slab_region md_bm_region md_count_v (G.reveal md_region_lv))
       (f_lemma size_class slab_region md_bm_region md_count_v (G.reveal md_region_lv))
-      (SeqUtils.init_u32_refined (U32.v md_count_v)))
+      (SeqUtils.init_us_refined (US.v md_count_v)))
     (left_vprop2 size_class slab_region md_bm_region md_count_v (G.reveal md_region_lv));
 
   intro_vdep
@@ -478,81 +479,81 @@ let pack_3
 
 let lemma_slab_aux_starseq
   (size_class: sc)
-  (slab_region: array U8.t{A.length slab_region = U32.v metadata_max * U32.v page_size})
-  (md_bm_region: array U64.t{A.length md_bm_region = U32.v metadata_max * 4})
-  (md_region: array AL.cell{A.length md_region = U32.v metadata_max})
-  (md_count_v: U32.t{U32.v md_count_v <= U32.v metadata_max})
-  (md_region_lv: G.erased (Seq.lseq AL.status (U32.v md_count_v)))
-  (idx:nat{idx < U32.v md_count_v})
+  (slab_region: array U8.t{A.length slab_region = US.v metadata_max * U32.v page_size})
+  (md_bm_region: array U64.t{A.length md_bm_region = US.v metadata_max * 4})
+  (md_region: array AL.cell{A.length md_region = US.v metadata_max})
+  (md_count_v: US.t{US.v md_count_v <= US.v metadata_max})
+  (md_region_lv: G.erased (Seq.lseq AL.status (US.v md_count_v)))
+  (idx:nat{idx < US.v md_count_v})
   (v:AL.status)
   : Lemma
   (let f1 = f size_class slab_region md_bm_region md_count_v md_region_lv in
    let f2 = f size_class slab_region md_bm_region md_count_v (Seq.upd (G.reveal md_region_lv) idx v) in
-   let s = SeqUtils.init_u32_refined (U32.v md_count_v) in
+   let s = SeqUtils.init_us_refined (US.v md_count_v) in
    forall (k:nat{k <> idx /\ k < Seq.length s}).
      f1 (Seq.index s k) == f2 (Seq.index s k))
   =
   let f1 = f size_class slab_region md_bm_region md_count_v md_region_lv in
   let f2 = f size_class slab_region md_bm_region md_count_v (Seq.upd (G.reveal md_region_lv) idx v) in
   let md_region_lv' = Seq.upd (G.reveal md_region_lv) idx v in
-  let s = SeqUtils.init_u32_refined (U32.v md_count_v) in
+  let s = SeqUtils.init_us_refined (US.v md_count_v) in
   let aux (k:nat{k <> idx /\ k < Seq.length s})
     : Lemma (f1 (Seq.index s k) == f2 (Seq.index s k))
     = let i = Seq.index s k in
-      SeqUtils.init_u32_refined_index (U32.v md_count_v) k;
-      assert (Seq.index md_region_lv (U32.v i) == Seq.index md_region_lv' (U32.v i))
+      SeqUtils.init_us_refined_index (US.v md_count_v) k;
+      assert (Seq.index md_region_lv (US.v i) == Seq.index md_region_lv' (US.v i))
   in Classical.forall_intro aux
 
 #push-options "--z3rlimit 75 --compat_pre_typed_indexed_effects"
 let pack_slab_starseq
   (#opened:_)
   (size_class: sc)
-  (slab_region: array U8.t{A.length slab_region = U32.v metadata_max * U32.v page_size})
-  (md_bm_region: array U64.t{A.length md_bm_region = U32.v metadata_max * 4})
-  (md_region: array AL.cell{A.length md_region = U32.v metadata_max})
-  (md_count: ref U32.t)
+  (slab_region: array U8.t{A.length slab_region = US.v metadata_max * U32.v page_size})
+  (md_bm_region: array U64.t{A.length md_bm_region = US.v metadata_max * 4})
+  (md_region: array AL.cell{A.length md_region = US.v metadata_max})
+  (md_count: ref US.t)
   (r1 r2 r3 r4: ref US.t)
-  (md_count_v: U32.t{U32.v md_count_v <= U32.v metadata_max})
-  (md_region_lv: G.erased (Seq.lseq AL.status (U32.v md_count_v)))
-  (idx: US.t{US.v idx < U32.v md_count_v})
+  (md_count_v: US.t{US.v md_count_v <= US.v metadata_max})
+  (md_region_lv: G.erased (Seq.lseq AL.status (US.v md_count_v)))
+  (idx: US.t{US.v idx < US.v md_count_v})
   (v: AL.status)
   : SteelGhost unit opened
   (
     slab_vprop size_class
-      (slab_array slab_region (US.sizet_to_uint32 idx))
-      (md_bm_array md_bm_region (US.sizet_to_uint32 idx)) `star`
+      (slab_array slab_region idx)
+      (md_bm_array md_bm_region idx) `star`
     (starseq
-      #(pos:U32.t{U32.v pos < U32.v md_count_v})
+      #(pos:US.t{US.v pos < US.v md_count_v})
       #(t size_class)
       (f size_class slab_region md_bm_region md_count_v md_region_lv)
       (f_lemma size_class slab_region md_bm_region md_count_v md_region_lv)
-      (Seq.slice (SeqUtils.init_u32_refined (U32.v md_count_v)) 0 (US.v idx)) `star`
+      (Seq.slice (SeqUtils.init_us_refined (US.v md_count_v)) 0 (US.v idx)) `star`
     starseq
-      #(pos:U32.t{U32.v pos < U32.v md_count_v})
+      #(pos:US.t{US.v pos < US.v md_count_v})
       #(t size_class)
       (f size_class slab_region md_bm_region md_count_v md_region_lv)
       (f_lemma size_class slab_region md_bm_region md_count_v md_region_lv)
-      (Seq.slice (SeqUtils.init_u32_refined (U32.v md_count_v)) (US.v idx + 1) (Seq.length (SeqUtils.init_u32_refined (U32.v md_count_v)))))
+      (Seq.slice (SeqUtils.init_us_refined (US.v md_count_v)) (US.v idx + 1) (Seq.length (SeqUtils.init_us_refined (US.v md_count_v)))))
   )
   (fun _ ->
     starseq
-      #(pos:U32.t{U32.v pos < U32.v md_count_v})
+      #(pos:US.t{US.v pos < US.v md_count_v})
       #(t size_class)
       (f size_class slab_region md_bm_region md_count_v (Seq.upd md_region_lv (US.v idx) v))
       (f_lemma size_class slab_region md_bm_region md_count_v (Seq.upd md_region_lv (US.v idx) v))
-      (SeqUtils.init_u32_refined (U32.v md_count_v))
+      (SeqUtils.init_us_refined (US.v md_count_v))
   )
   (requires fun h0 ->
     let md_blob : t_of (slab_vprop size_class
-      (slab_array slab_region (US.sizet_to_uint32 idx))
-      (md_bm_array md_bm_region (US.sizet_to_uint32 idx)))
+      (slab_array slab_region idx)
+      (md_bm_array md_bm_region idx))
     = h0 (slab_vprop size_class
-      (slab_array slab_region (US.sizet_to_uint32 idx))
-      (md_bm_array md_bm_region (US.sizet_to_uint32 idx))) in
+      (slab_array slab_region idx)
+      (md_bm_array md_bm_region idx)) in
     let md : Seq.lseq U64.t 4 = dfst (fst md_blob) in
     (v == 3ul ==> is_guard size_class
-      (slab_array slab_region (US.sizet_to_uint32 idx))
-      (md_bm_array md_bm_region (US.sizet_to_uint32 idx)) md_blob) /\
+      (slab_array slab_region idx)
+      (md_bm_array md_bm_region idx) md_blob) /\
     (v == 2ul ==> is_full size_class md) /\
     (v == 1ul ==> is_partial size_class md) /\
     (v == 0ul ==> is_empty size_class md) /\
@@ -560,61 +561,61 @@ let pack_slab_starseq
   )
   (ensures fun h0 _ h1 -> True)
   =
-  SeqUtils.init_u32_refined_index (U32.v md_count_v) (US.v idx);
+  SeqUtils.init_us_refined_index (US.v md_count_v) (US.v idx);
   if U32.eq v 3ul then (
     p_guard_pack size_class
-      (md_bm_array md_bm_region (US.sizet_to_uint32 idx),
-      slab_array slab_region (US.sizet_to_uint32 idx))
-      (md_bm_array md_bm_region (US.sizet_to_uint32 idx),
-      slab_array slab_region (US.sizet_to_uint32 idx));
+      (md_bm_array md_bm_region idx,
+      slab_array slab_region idx)
+      (md_bm_array md_bm_region idx,
+      slab_array slab_region idx);
     change_equal_slprop
-      (p_guard size_class (md_bm_array md_bm_region (US.sizet_to_uint32 idx), slab_array slab_region (US.sizet_to_uint32 idx)))
+      (p_guard size_class (md_bm_array md_bm_region idx, slab_array slab_region idx))
       (f size_class slab_region md_bm_region md_count_v (Seq.upd md_region_lv (US.v idx) v)
-        (Seq.index (SeqUtils.init_u32_refined (U32.v md_count_v)) (US.v idx)))
+        (Seq.index (SeqUtils.init_us_refined (US.v md_count_v)) (US.v idx)))
   ) else if U32.eq v 2ul then (
     p_full_pack size_class
-      (md_bm_array md_bm_region (US.sizet_to_uint32 idx),
-      slab_array slab_region (US.sizet_to_uint32 idx))
-      (md_bm_array md_bm_region (US.sizet_to_uint32 idx),
-      slab_array slab_region (US.sizet_to_uint32 idx));
+      (md_bm_array md_bm_region idx,
+      slab_array slab_region idx)
+      (md_bm_array md_bm_region idx,
+      slab_array slab_region idx);
     change_equal_slprop
-      (p_full size_class (md_bm_array md_bm_region (US.sizet_to_uint32 idx), slab_array slab_region (US.sizet_to_uint32 idx)))
+      (p_full size_class (md_bm_array md_bm_region idx, slab_array slab_region idx))
       (f size_class slab_region md_bm_region md_count_v (Seq.upd md_region_lv (US.v idx) v)
-        (Seq.index (SeqUtils.init_u32_refined (U32.v md_count_v)) (US.v idx)))
+        (Seq.index (SeqUtils.init_us_refined (US.v md_count_v)) (US.v idx)))
   ) else if U32.eq v 1ul then (
     p_partial_pack size_class
-      (md_bm_array md_bm_region (US.sizet_to_uint32 idx),
-      slab_array slab_region (US.sizet_to_uint32 idx))
-      (md_bm_array md_bm_region (US.sizet_to_uint32 idx),
-      slab_array slab_region (US.sizet_to_uint32 idx));
+      (md_bm_array md_bm_region idx,
+      slab_array slab_region idx)
+      (md_bm_array md_bm_region idx,
+      slab_array slab_region idx);
     change_equal_slprop
-      (p_partial size_class (md_bm_array md_bm_region (US.sizet_to_uint32 idx), slab_array slab_region (US.sizet_to_uint32 idx)))
+      (p_partial size_class (md_bm_array md_bm_region idx, slab_array slab_region idx))
       (f size_class slab_region md_bm_region md_count_v (Seq.upd md_region_lv (US.v idx) v)
-        (Seq.index (SeqUtils.init_u32_refined (U32.v md_count_v)) (US.v idx)))
+        (Seq.index (SeqUtils.init_us_refined (US.v md_count_v)) (US.v idx)))
   ) else (
      p_empty_pack size_class
-      (md_bm_array md_bm_region (US.sizet_to_uint32 idx),
-      slab_array slab_region (US.sizet_to_uint32 idx))
-      (md_bm_array md_bm_region (US.sizet_to_uint32 idx),
-      slab_array slab_region (US.sizet_to_uint32 idx));
+      (md_bm_array md_bm_region idx,
+      slab_array slab_region idx)
+      (md_bm_array md_bm_region idx,
+      slab_array slab_region idx);
     change_equal_slprop
-      (p_empty size_class (md_bm_array md_bm_region (US.sizet_to_uint32 idx), slab_array slab_region (US.sizet_to_uint32 idx)))
+      (p_empty size_class (md_bm_array md_bm_region idx, slab_array slab_region idx))
       (f size_class slab_region md_bm_region md_count_v (Seq.upd md_region_lv (US.v idx) v)
-        (Seq.index (SeqUtils.init_u32_refined (U32.v md_count_v)) (US.v idx)))
+        (Seq.index (SeqUtils.init_us_refined (US.v md_count_v)) (US.v idx)))
   );
   lemma_slab_aux_starseq size_class
     slab_region md_bm_region md_region
     md_count_v md_region_lv (US.v idx) v;
   starseq_upd_pack
     #_
-    #(pos:U32.t{U32.v pos < U32.v md_count_v})
+    #(pos:US.t{US.v pos < US.v md_count_v})
     #(t size_class)
     (f size_class slab_region md_bm_region md_count_v md_region_lv)
     (f size_class slab_region md_bm_region md_count_v (Seq.upd (G.reveal md_region_lv) (US.v idx) v))
     (f_lemma size_class slab_region md_bm_region md_count_v md_region_lv)
     (f_lemma size_class slab_region md_bm_region md_count_v (Seq.upd (G.reveal md_region_lv) (US.v idx) v))
-    (SeqUtils.init_u32_refined (U32.v md_count_v))
-    (SeqUtils.init_u32_refined (U32.v md_count_v))
+    (SeqUtils.init_us_refined (US.v md_count_v))
+    (SeqUtils.init_us_refined (US.v md_count_v))
     (US.v idx)
 #pop-options
 
@@ -622,12 +623,12 @@ let pack_slab_starseq
 let pack_right_and_refactor_vrefine_dep
   (#opened:_)
   (size_class: sc)
-  (slab_region: array U8.t{A.length slab_region = U32.v metadata_max * U32.v page_size})
-  (md_bm_region: array U64.t{A.length md_bm_region = U32.v metadata_max * 4})
-  (md_region: array AL.cell{A.length md_region = U32.v metadata_max})
-  (md_count: ref U32.t)
+  (slab_region: array U8.t{A.length slab_region = US.v metadata_max * U32.v page_size})
+  (md_bm_region: array U64.t{A.length md_bm_region = US.v metadata_max * 4})
+  (md_region: array AL.cell{A.length md_region = US.v metadata_max})
+  (md_count: ref US.t)
   (r1 r2 r3 r4: ref US.t)
-  (md_count_v: U32.t{U32.v md_count_v <= U32.v metadata_max})
+  (md_count_v: US.t{US.v md_count_v <= US.v metadata_max})
   : SteelGhost unit opened
   (
     vrefinedep
