src/SlabsCommon.fsti
@@ -311,65 +311,65 @@ val p_guard_pack (#opened:_)
 /// Retrieving the slab at index [md_count] in the [slab_region]
 inline_for_extraction noextract
 val slab_array
-  (slab_region: array U8.t{A.length slab_region = U32.v metadata_max * U32.v page_size})
-  (md_count: U32.t{U32.v md_count < U32.v metadata_max})
+  (slab_region: array U8.t{A.length slab_region = US.v metadata_max * U32.v page_size})
+  (md_count: US.t{US.v md_count < US.v metadata_max})
   : Pure (array U8.t)
   (requires
-    A.length slab_region = U32.v metadata_max * U32.v page_size /\
-    U32.v md_count < U32.v metadata_max)
+    A.length slab_region = US.v metadata_max * U32.v page_size /\
+    US.v md_count < US.v metadata_max)
   (ensures fun r ->
     A.length r = U32.v page_size /\
     same_base_array r slab_region /\
-    A.offset (A.ptr_of r) == A.offset (A.ptr_of slab_region) + U32.v md_count * U32.v page_size
+    A.offset (A.ptr_of r) == A.offset (A.ptr_of slab_region) + US.v md_count * U32.v page_size
   )
 
 #push-options "--print_implicits"
 
 val pack_slab_array (#opened:_)
-  (slab_region: array U8.t{A.length slab_region = U32.v metadata_max * U32.v page_size})
-  (md_count: U32.t{U32.v md_count < U32.v metadata_max})
+  (slab_region: array U8.t{A.length slab_region = US.v metadata_max * U32.v page_size})
+  (md_count: US.t{US.v md_count < US.v metadata_max})
   : SteelGhost unit opened
-    (A.varray (A.split_l (A.split_r slab_region (u32_to_sz (U32.mul md_count page_size))) (u32_to_sz page_size)))
+    (A.varray (A.split_l (A.split_r slab_region (US.mul md_count (u32_to_sz page_size))) (u32_to_sz page_size)))
     (fun _ -> A.varray (slab_array slab_region md_count))
     (requires fun _ -> True)
     (ensures fun h0 _ h1 ->
-      A.asel (A.split_l (A.split_r slab_region (u32_to_sz (U32.mul md_count page_size))) (u32_to_sz page_size)) h0 ==
+      A.asel (A.split_l (A.split_r slab_region (US.mul md_count (u32_to_sz page_size))) (u32_to_sz page_size)) h0 ==
       A.asel (slab_array slab_region md_count) h1)
 
 /// Retrieving the metadata bitmap at index [md_count] in array [md_bm_region]
 inline_for_extraction noextract
 val md_bm_array
-  (md_bm_region: array U64.t{A.length md_bm_region = U32.v metadata_max * 4})
-  (md_count: U32.t{U32.v md_count < U32.v metadata_max})
+  (md_bm_region: array U64.t{A.length md_bm_region = US.v metadata_max * 4})
+  (md_count: US.t{US.v md_count < US.v metadata_max})
   : Pure (array U64.t)
   (requires
-    A.length md_bm_region = U32.v metadata_max * 4 /\
-    U32.v md_count < U32.v metadata_max)
+    A.length md_bm_region = US.v metadata_max * 4 /\
+    US.v md_count < US.v metadata_max)
   (ensures fun r ->
     A.length r = 4 /\
     same_base_array r md_bm_region
   )
 
 val pack_md_bm_array (#opened:_)
-  (md_bm_region: array U64.t{A.length md_bm_region = U32.v metadata_max * 4})
-  (md_count: U32.t{U32.v md_count < U32.v metadata_max})
+  (md_bm_region: array U64.t{A.length md_bm_region = US.v metadata_max * 4})
+  (md_count: US.t{US.v md_count < US.v metadata_max})
   : SteelGhost unit opened
-    (A.varray (A.split_l (A.split_r md_bm_region (u32_to_sz (U32.mul md_count 4ul))) (u32_to_sz 4ul)))
+    (A.varray (A.split_l (A.split_r md_bm_region (US.mul md_count 4sz)) 4sz))
     (fun _ -> A.varray (md_bm_array md_bm_region md_count))
     (requires fun _ -> True)
     (ensures fun h0 _ h1 ->
-      A.asel (A.split_l (A.split_r md_bm_region (u32_to_sz (U32.mul md_count 4ul))) (u32_to_sz 4ul)) h0 ==
+      A.asel (A.split_l (A.split_r md_bm_region (US.mul md_count 4sz)) 4sz) h0 ==
       A.asel (md_bm_array md_bm_region md_count) h1)
 
 /// Retrieving the metadata status indicator at index [md_count] in array [md_region]
 inline_for_extraction noextract
 val md_array
-  (md_region: array AL.cell{A.length md_region = U32.v metadata_max})
-  (md_count: U32.t{U32.v md_count < U32.v metadata_max})
+  (md_region: array AL.cell{A.length md_region = US.v metadata_max})
+  (md_count: US.t{US.v md_count < US.v metadata_max})
   : Pure (array AL.cell)
   (requires
-    A.length md_region = U32.v metadata_max /\
-    U32.v md_count < U32.v metadata_max)
+    A.length md_region = US.v metadata_max /\
+    US.v md_count < US.v metadata_max)
   (ensures fun r ->
     A.length r = 1 /\
     same_base_array r md_region /\
@@ -377,25 +377,25 @@ val md_array
   )
 
 val pack_md_array (#opened:_)
-  (md_region: array AL.cell{A.length md_region = U32.v metadata_max})
-  (md_count: U32.t{U32.v md_count < U32.v metadata_max})
+  (md_region: array AL.cell{A.length md_region = US.v metadata_max})
+  (md_count: US.t{US.v md_count < US.v metadata_max})
   : SteelGhost unit opened
-    (A.varray (A.split_l (A.split_r md_region (u32_to_sz md_count)) (u32_to_sz 1ul)))
+    (A.varray (A.split_l (A.split_r md_region md_count) 1sz))
     (fun _ -> A.varray (md_array md_region md_count))
     (requires fun _ -> True)
     (ensures fun h0 _ h1 ->
-      A.asel (A.split_l (A.split_r md_region (u32_to_sz md_count)) (u32_to_sz 1ul)) h0 ==
+      A.asel (A.split_l (A.split_r md_region md_count) 1sz) h0 ==
       A.asel (md_array md_region md_count) h1)
 
 val unpack_md_array (#opened:_)
-  (md_region: array AL.cell{A.length md_region = U32.v metadata_max})
-  (md_count: U32.t{U32.v md_count < U32.v metadata_max})
+  (md_region: array AL.cell{A.length md_region = US.v metadata_max})
+  (md_count: US.t{US.v md_count < US.v metadata_max})
   : SteelGhost unit opened
     (A.varray (md_array md_region md_count))
-    (fun _ -> A.varray (A.split_l (A.split_r md_region (u32_to_sz md_count)) 1sz))
+    (fun _ -> A.varray (A.split_l (A.split_r md_region md_count) 1sz))
     (requires fun _ -> True)
     (ensures fun h0 _ h1 ->
-      A.asel (A.split_l (A.split_r md_region (u32_to_sz md_count)) 1sz) h1 ==
+      A.asel (A.split_l (A.split_r md_region md_count) 1sz) h1 ==
       A.asel (md_array md_region md_count) h0)
 
 (** VProps related to slabs *)
@@ -404,14 +404,14 @@ val unpack_md_array (#opened:_)
 
 let f
   (size_class: sc)
-  (slab_region: array U8.t{A.length slab_region = U32.v metadata_max * U32.v page_size})
-  (md_bm_region: array U64.t{A.length md_bm_region = U32.v metadata_max * 4})
-  (md_count_v: U32.t{U32.v md_count_v <= U32.v metadata_max})
-  (md_region_lv: Seq.lseq AL.status (U32.v md_count_v))
-  (i: U32.t{U32.v i < U32.v md_count_v})
+  (slab_region: array U8.t{A.length slab_region = US.v metadata_max * U32.v page_size})
+  (md_bm_region: array U64.t{A.length md_bm_region = US.v metadata_max * 4})
+  (md_count_v: US.t{US.v md_count_v <= US.v metadata_max})
+  (md_region_lv: Seq.lseq AL.status (US.v md_count_v))
+  (i: US.t{US.v i < US.v md_count_v})
   : vprop
   =
-  match Seq.index md_region_lv (U32.v i) with
+  match Seq.index md_region_lv (US.v i) with
   | 0ul -> p_empty size_class (md_bm_array md_bm_region i, slab_array slab_region i)
   | 1ul -> p_partial size_class (md_bm_array md_bm_region i, slab_array slab_region i)
   | 2ul -> p_full size_class (md_bm_array md_bm_region i, slab_array slab_region i)
@@ -421,11 +421,11 @@ val t (size_class: sc) : Type0
 
 val f_lemma
   (size_class: sc)
-  (slab_region: array U8.t{A.length slab_region = U32.v metadata_max * U32.v page_size})
-  (md_bm_region: array U64.t{A.length md_bm_region = U32.v metadata_max * 4})
-  (md_count_v: U32.t{U32.v md_count_v <= U32.v metadata_max})
-  (md_region_lv: Seq.lseq AL.status (U32.v md_count_v))
-  (i: U32.t{U32.v i < U32.v md_count_v})
+  (slab_region: array U8.t{A.length slab_region = US.v metadata_max * U32.v page_size})
+  (md_bm_region: array U64.t{A.length md_bm_region = US.v metadata_max * 4})
+  (md_count_v: US.t{US.v md_count_v <= US.v metadata_max})
+  (md_region_lv: Seq.lseq AL.status (US.v md_count_v))
+  (i: US.t{US.v i < US.v md_count_v})
   : Lemma
   (t_of (f size_class slab_region md_bm_region md_count_v md_region_lv i)
   == t size_class)
@@ -468,80 +468,80 @@ let ind_varraylist
   ind_varraylist_aux pred1 pred2 pred3 pred4 r
 
 let left_vprop1
-  (md_region: array AL.cell{A.length md_region = U32.v metadata_max})
+  (md_region: array AL.cell{A.length md_region = US.v metadata_max})
   (r1 r2 r3 r4: ref US.t)
-  (md_count_v: U32.t{U32.v md_count_v <= U32.v metadata_max})
+  (md_count_v: US.t{US.v md_count_v <= US.v metadata_max})
   =
   ind_varraylist pred1 pred2 pred3 pred4
-    (A.split_l md_region (u32_to_sz md_count_v))
+    (A.split_l md_region md_count_v)
     r1 r2 r3 r4
 
 let left_vprop2
   (size_class: sc)
-  (slab_region: array U8.t{A.length slab_region = U32.v metadata_max * U32.v page_size})
-  (md_bm_region: array U64.t{A.length md_bm_region = U32.v metadata_max * 4})
-  (md_count_v: U32.t{U32.v md_count_v <= U32.v metadata_max})
-  (x: Seq.lseq AL.status (U32.v md_count_v))
+  (slab_region: array U8.t{A.length slab_region = US.v metadata_max * U32.v page_size})
+  (md_bm_region: array U64.t{A.length md_bm_region = US.v metadata_max * 4})
+  (md_count_v: US.t{US.v md_count_v <= US.v metadata_max})
+  (x: Seq.lseq AL.status (US.v md_count_v))
   =
   starseq
-    #(pos:U32.t{U32.v pos < U32.v md_count_v})
+    #(pos:US.t{US.v pos < US.v md_count_v})
     #(t size_class)
     (f size_class slab_region md_bm_region md_count_v x)
     (f_lemma size_class slab_region md_bm_region md_count_v x)
-    (SeqUtils.init_u32_refined (U32.v md_count_v))
+    (SeqUtils.init_us_refined (US.v md_count_v))
 
 let left_vprop_aux
   (size_class: sc)
-  (slab_region: array U8.t{A.length slab_region = U32.v metadata_max * U32.v page_size})
-  (md_bm_region: array U64.t{A.length md_bm_region = U32.v metadata_max * 4})
-  (md_region: array AL.cell{A.length md_region = U32.v metadata_max})
+  (slab_region: array U8.t{A.length slab_region = US.v metadata_max * U32.v page_size})
+  (md_bm_region: array U64.t{A.length md_bm_region = US.v metadata_max * 4})
+  (md_region: array AL.cell{A.length md_region = US.v metadata_max})
   (r1 r2 r3 r4: ref US.t)
-  (md_count_v: U32.t{U32.v md_count_v <= U32.v metadata_max})
-  (x: t_of (ind_varraylist pred1 pred2 pred3 pred4 (A.split_l md_region (u32_to_sz md_count_v)) r1 r2 r3 r4))
+  (md_count_v: US.t{US.v md_count_v <= US.v metadata_max})
+  (x: t_of (ind_varraylist pred1 pred2 pred3 pred4 (A.split_l md_region md_count_v) r1 r2 r3 r4))
   = starseq
-      #(pos:U32.t{U32.v pos < U32.v md_count_v})
+      #(pos:US.t{US.v pos < US.v md_count_v})
       #(t size_class)
       (f size_class slab_region md_bm_region md_count_v (ALG.dataify (dsnd x)))
       (f_lemma size_class slab_region md_bm_region md_count_v (ALG.dataify (dsnd x)))
-      (SeqUtils.init_u32_refined (U32.v md_count_v))
+      (SeqUtils.init_us_refined (US.v md_count_v))
 
 let left_vprop
   (size_class: sc)
-  (slab_region: array U8.t{A.length slab_region = U32.v metadata_max * U32.v page_size})
-  (md_bm_region: array U64.t{A.length md_bm_region = U32.v metadata_max * 4})
-  (md_region: array AL.cell{A.length md_region = U32.v metadata_max})
+  (slab_region: array U8.t{A.length slab_region = US.v metadata_max * U32.v page_size})
+  (md_bm_region: array U64.t{A.length md_bm_region = US.v metadata_max * 4})
+  (md_region: array AL.cell{A.length md_region = US.v metadata_max})
   (r1 r2 r3 r4: ref US.t)
-  (md_count_v: U32.t{U32.v md_count_v <= U32.v metadata_max})
+  (md_count_v: US.t{US.v md_count_v <= US.v metadata_max})
   =
   left_vprop1 md_region r1 r2 r3 r4 md_count_v
   `vdep`
   left_vprop_aux size_class slab_region md_bm_region md_region r1 r2 r3 r4 md_count_v
 
 unfold
-let vrefinedep_prop (x:U32.t) : prop =
-  U32.v x <= U32.v metadata_max /\
-  U32.v x <> AL.null
+let vrefinedep_prop (x:US.t) : prop =
+  US.v x <= US.v metadata_max /\
+  US.v x <> AL.null
 
 let right_vprop
-  (slab_region: array U8.t{A.length slab_region = U32.v metadata_max * U32.v page_size})
-  (md_bm_region: array U64.t{A.length md_bm_region = U32.v metadata_max * 4})
-  (md_region: array AL.cell{A.length md_region = U32.v metadata_max})
-  (v: U32.t{U32.v v <= U32.v metadata_max})
+  (slab_region: array U8.t{A.length slab_region = US.v metadata_max * U32.v page_size})
+  (md_bm_region: array U64.t{A.length md_bm_region = US.v metadata_max * 4})
+  (md_region: array AL.cell{A.length md_region = US.v metadata_max})
+  (v: US.t{US.v v <= US.v metadata_max})
   : vprop
   =
-  (A.varray (A.split_r slab_region (u32_to_sz (U32.mul v page_size)))
+  (A.varray (A.split_r slab_region (US.mul v (u32_to_sz page_size)))
     `vrefine` zf_u8) `star`
-  (A.varray (A.split_r md_bm_region (u32_to_sz (U32.mul v 4ul)))
+  (A.varray (A.split_r md_bm_region (US.mul v 4sz))
     `vrefine` zf_u64) `star`
-  A.varray (A.split_r md_region (u32_to_sz v))
+  A.varray (A.split_r md_region v)
 
 let size_class_vprop_aux
   (size_class: sc)
-  (slab_region: array U8.t{A.length slab_region = U32.v metadata_max * U32.v page_size})
-  (md_bm_region: array U64.t{A.length md_bm_region = U32.v metadata_max * 4})
-  (md_region: array AL.cell{A.length md_region = U32.v metadata_max})
+  (slab_region: array U8.t{A.length slab_region = US.v metadata_max * U32.v page_size})
+  (md_bm_region: array U64.t{A.length md_bm_region = US.v metadata_max * 4})
+  (md_region: array AL.cell{A.length md_region = US.v metadata_max})
   empty_slabs partial_slabs full_slabs guard_slabs
-  (v: U32.t{U32.v v <= U32.v metadata_max == true})
+  (v: US.t{US.v v <= US.v metadata_max == true})
   : vprop
   =
   left_vprop size_class
@@ -556,13 +556,13 @@ open SteelVRefineDep
 val pack_3
   (#opened:_)
   (size_class: sc)
-  (slab_region: array U8.t{A.length slab_region = U32.v metadata_max * U32.v page_size})
-  (md_bm_region: array U64.t{A.length md_bm_region = U32.v metadata_max * 4})
-  (md_region: array AL.cell{A.length md_region = U32.v metadata_max})
-  (md_count: ref U32.t)
+  (slab_region: array U8.t{A.length slab_region = US.v metadata_max * U32.v page_size})
+  (md_bm_region: array U64.t{A.length md_bm_region = US.v metadata_max * 4})
+  (md_region: array AL.cell{A.length md_region = US.v metadata_max})
+  (md_count: ref US.t)
   (r1 r2 r3 r4: ref US.t)
-  (md_count_v: U32.t{U32.v md_count_v <= U32.v metadata_max})
-  (md_region_lv: G.erased (Seq.lseq AL.status (U32.v md_count_v)))
+  (md_count_v: US.t{US.v md_count_v <= US.v metadata_max})
+  (md_region_lv: G.erased (Seq.lseq AL.status (US.v md_count_v)))
   (idx1 idx2 idx3 idx4: US.t)
   : SteelGhost unit opened
   (
@@ -572,14 +572,14 @@ val pack_3
     vptr r3 `star`
     vptr r4 `star`
     (AL.varraylist pred1 pred2 pred3 pred4
-      (A.split_l md_region (u32_to_sz md_count_v))
+      (A.split_l md_region md_count_v)
       (US.v idx1) (US.v idx2) (US.v idx3) (US.v idx4)) `star`
     starseq
-      #(pos:U32.t{U32.v pos < U32.v md_count_v})
+      #(pos:US.t{US.v pos < US.v md_count_v})
       #(t size_class)
       (f size_class slab_region md_bm_region md_count_v (G.reveal md_region_lv))
       (f_lemma size_class slab_region md_bm_region md_count_v (G.reveal md_region_lv))
-      (SeqUtils.init_u32_refined (U32.v md_count_v))
+      (SeqUtils.init_us_refined (US.v md_count_v))
   )
   (fun _ ->
     vrefinedep
@@ -589,9 +589,9 @@ val pack_3
   )
   (requires fun h0 ->
     let gs0 = AL.v_arraylist pred1 pred2 pred3 pred4
-      (A.split_l md_region (u32_to_sz md_count_v))
+      (A.split_l md_region md_count_v)
       (US.v idx1) (US.v idx2) (US.v idx3) (US.v idx4) h0 in
-    U32.v md_count_v <> AL.null /\
+    US.v md_count_v <> AL.null /\
     sel md_count h0 == md_count_v /\
     sel r1 h0 == idx1 /\
     sel r2 h0 == idx2 /\
@@ -613,53 +613,53 @@ val pack_3
 val pack_slab_starseq
   (#opened:_)
   (size_class: sc)
-  (slab_region: array U8.t{A.length slab_region = U32.v metadata_max * U32.v page_size})
-  (md_bm_region: array U64.t{A.length md_bm_region = U32.v metadata_max * 4})
-  (md_region: array AL.cell{A.length md_region = U32.v metadata_max})
-  (md_count: ref U32.t)
+  (slab_region: array U8.t{A.length slab_region = US.v metadata_max * U32.v page_size})
+  (md_bm_region: array U64.t{A.length md_bm_region = US.v metadata_max * 4})
+  (md_region: array AL.cell{A.length md_region = US.v metadata_max})
+  (md_count: ref US.t)
   (r1 r2 r3 r4: ref US.t)
-  (md_count_v: U32.t{U32.v md_count_v <= U32.v metadata_max})
-  (md_region_lv: G.erased (Seq.lseq AL.status (U32.v md_count_v)))
-  (idx: US.t{US.v idx < U32.v md_count_v})
+  (md_count_v: US.t{US.v md_count_v <= US.v metadata_max})
+  (md_region_lv: G.erased (Seq.lseq AL.status (US.v md_count_v)))
+  (idx: US.t{US.v idx < US.v md_count_v})
   (v: AL.status)
   : SteelGhost unit opened
   (
     slab_vprop size_class
-      (slab_array slab_region (US.sizet_to_uint32 idx))
-      (md_bm_array md_bm_region (US.sizet_to_uint32 idx)) `star`
+      (slab_array slab_region idx)
+      (md_bm_array md_bm_region idx) `star`
     (starseq
-      #(pos:U32.t{U32.v pos < U32.v md_count_v})
+      #(pos:US.t{US.v pos < US.v md_count_v})
       #(t size_class)
       (f size_class slab_region md_bm_region md_count_v md_region_lv)
       (f_lemma size_class slab_region md_bm_region md_count_v md_region_lv)
-      (Seq.slice (SeqUtils.init_u32_refined (U32.v md_count_v)) 0 (US.v idx)) `star`
+      (Seq.slice (SeqUtils.init_us_refined (US.v md_count_v)) 0 (US.v idx)) `star`
     starseq
-      #(pos:U32.t{U32.v pos < U32.v md_count_v})
+      #(pos:US.t{US.v pos < US.v md_count_v})
       #(t size_class)
       (f size_class slab_region md_bm_region md_count_v md_region_lv)
       (f_lemma size_class slab_region md_bm_region md_count_v md_region_lv)
-      (Seq.slice (SeqUtils.init_u32_refined (U32.v md_count_v)) (US.v idx + 1) (Seq.length (SeqUtils.init_u32_refined (U32.v md_count_v)))))
+      (Seq.slice (SeqUtils.init_us_refined (US.v md_count_v)) (US.v idx + 1) (Seq.length (SeqUtils.init_us_refined (US.v md_count_v)))))
   )
   (fun _ ->
     starseq
-      #(pos:U32.t{U32.v pos < U32.v md_count_v})
+      #(pos:US.t{US.v pos < US.v md_count_v})
       #(t size_class)
       (f size_class slab_region md_bm_region md_count_v (Seq.upd md_region_lv (US.v idx) v))
       (f_lemma size_class slab_region md_bm_region md_count_v (Seq.upd md_region_lv (US.v idx) v))
-      (SeqUtils.init_u32_refined (U32.v md_count_v))
+      (SeqUtils.init_us_refined (US.v md_count_v))
   )
   (requires fun h0 ->
     let md_blob : t_of (slab_vprop size_class
-      (slab_array slab_region (US.sizet_to_uint32 idx))
-      (md_bm_array md_bm_region (US.sizet_to_uint32 idx)))
+      (slab_array slab_region idx)
+      (md_bm_array md_bm_region idx))
     = h0 (slab_vprop size_class
-      (slab_array slab_region (US.sizet_to_uint32 idx))
-      (md_bm_array md_bm_region (US.sizet_to_uint32 idx))) in
+      (slab_array slab_region idx)
+      (md_bm_array md_bm_region idx)) in
     let md : Seq.lseq U64.t 4 = dfst (fst md_blob) in
     //(v == 3ul ==> is_guard size_class md) /\
     (v == 3ul ==> is_guard size_class
-      (slab_array slab_region (US.sizet_to_uint32 idx))
-      (md_bm_array md_bm_region (US.sizet_to_uint32 idx)) md_blob) /\
+      (slab_array slab_region idx)
+      (md_bm_array md_bm_region idx) md_blob) /\
     (v == 2ul ==> is_full size_class md) /\
     (v == 1ul ==> is_partial size_class md) /\
     (v == 0ul ==> is_empty size_class md) /\
@@ -670,12 +670,12 @@ val pack_slab_starseq
 val pack_right_and_refactor_vrefine_dep
   (#opened:_)
   (size_class: sc)
-  (slab_region: array U8.t{A.length slab_region = U32.v metadata_max * U32.v page_size})
-  (md_bm_region: array U64.t{A.length md_bm_region = U32.v metadata_max * 4})
-  (md_region: array AL.cell{A.length md_region = U32.v metadata_max})
-  (md_count: ref U32.t)
+  (slab_region: array U8.t{A.length slab_region = US.v metadata_max * U32.v page_size})
+  (md_bm_region: array U64.t{A.length md_bm_region = US.v metadata_max * 4})
+  (md_region: array AL.cell{A.length md_region = US.v metadata_max})
+  (md_count: ref US.t)
   (r1 r2 r3 r4: ref US.t)
-  (md_count_v: U32.t{U32.v md_count_v <= U32.v metadata_max})
+  (md_count_v: US.t{US.v md_count_v <= US.v metadata_max})
   : SteelGhost unit opened
   (
     vrefinedep
